Separated PermutationRules.v and Permutations.v into a number of smaller files in the folder src/Permutations, in preperation for moving some of them to QuantumLib. This commit builds, but naming is poor.

src/Permutations/ZXperm.v
@@ -1,38 +1,36 @@
-Require Import ZXCore.
-Require Import QuantumLib.Permutations.
+Require Import CoreData.ZXCore.
+Require Import PermutationDefinitions.
 
 Open Scope ZX_scope.
 
-Inductive ZX_Perm : forall n m, ZX n m -> Prop :=
-  | PermEmpty : ZX_Perm 0 0 Empty
-  | PermWire : ZX_Perm 1 1 Wire
-  | PermSwap : ZX_Perm 2 2 ⨉
+(* @nocheck name *)
+(* Allowing combination of Z and X; will check before push *)
+Inductive ZXperm : forall n m, ZX n m -> Prop :=
+  | PermEmpty : ZXperm 0 0 Empty
+  | PermWire : ZXperm 1 1 Wire
+  | PermSwap : ZXperm 2 2 ⨉
   | PermStack {n0 m0 n1 m1 zx0 zx1} : 
-      (ZX_Perm n0 m0 zx0) -> (ZX_Perm n1 m1 zx1) -> ZX_Perm _ _ (zx0 ↕ zx1)
+      (ZXperm n0 m0 zx0) -> (ZXperm n1 m1 zx1) -> ZXperm _ _ (zx0 ↕ zx1)
   | PermComp {n m o zx0 zx1} : 
-      (ZX_Perm n m zx0) -> (ZX_Perm m o zx1) -> ZX_Perm _ _ (zx0 ⟷ zx1).
+      (ZXperm n m zx0) -> (ZXperm m o zx1) -> ZXperm _ _ (zx0 ⟷ zx1).
 
-Definition swap_permutation : nat -> nat :=
-  fun n => match n with
-    | 0 => 1%nat
-    | 1 => 0%nat
-    | other => other
-  end.
-
-Definition stack_permutations (n0 n1 : nat) (f g : nat -> nat) : nat -> nat :=
+(*
+TODO: Bring this back here?
+Definition stack_perms (n0 n1 : nat) (f g : nat -> nat) : nat -> nat :=
   fun n => if (n <? n0) then f n else 
            if (n <? n0 + n1) then (g (n - n0) + n0)%nat else n.
+*)
 
 Fixpoint perm_of_zx {n m} (zx : ZX n m) : (nat -> nat) :=
   let idn := (fun x : nat => x) in
     match zx with 
     | Empty => idn
     | Wire => idn
-    | Swap => swap_permutation
+    | Swap => swap_2_perm
     | @Compose n m o zx0 zx1 =>
         ((perm_of_zx zx0) ∘ (perm_of_zx zx1))%prg
     | @Stack n0 m0 n1 m1 zx0 zx1 =>
-        stack_permutations n0 n1 (perm_of_zx zx0) (perm_of_zx zx1)
+        stack_perms n0 n1 (perm_of_zx zx0) (perm_of_zx zx1)
     (* Fake cases: *)
     | Cap => idn
     | Cup => idn
@@ -54,8 +52,4 @@ Definition top_to_bottom_perm (n : nat) : nat -> nat :=
 	fun k => if n <=? k then k else
 	         if k =? (n-1) then 0%nat else (k + 1)%nat.
 
-Definition rotr n m : nat -> nat :=
-	fun k => if n <=? k then k else (k + m) mod n.
 
-Definition rotl n m : nat -> nat :=
-	fun k => if n <=? k then k else (k + (n - (m mod n))) mod n.
