src/CoreData/CoreData.v
@@ -3,4 +3,4 @@ Require Export Proportional.
 Require Export Swaps.
 Require Export StrongInduction.
 Require Export CapCup.
-Require Export Permutations.
+(* Require Export Permutations. *)
