src/Permutations/PermutationAutomation.v
@@ -1,0 +1,177 @@
+Require Export CoreData.ZXCore.
+Require Export PermutationDefinitions.
+Require Export QuantumLib.Permutations.
+Require Export CoreRules.CoreAutomation.
+
+(* TODOs: 
+    - Declare databases
+    - Remove all these random tactics; replace with the standard ones
+*)
+
+Tactic Notation "tryeasylia" :=
+  try easy; try lia.
+
+Ltac bdest_lia_replace b0 b1 :=
+  replace b0 with b1 by (bdestruct b0; lia).
+
+Ltac show_permutation :=
+  repeat first [
+    split
+  | simpl; solve [auto with perm_db]
+  | subst; solve [auto with perm_db]
+  | auto with perm_db
+  | solve [eauto using permutation_compose with perm_db]
+  | easy
+  | lia
+  ].
+
+Ltac enumerate_value i :=
+  destruct i; [|tryif lia then idtac else enumerate_value i].
+
+Ltac enumerate_matrix Hi Hj :=
+  match type of Hi with (?i < ?n)%nat =>
+  match type of Hj with (?j < ?m)%nat => 
+  enumerate_value i; enumerate_value j
+  (* repeat first [destruct i; destruct j; try lia] *)
+  end end.
+
+  (* by_cell *)
+
+Ltac check_finite_matrix :=
+  apply mat_equiv_eq;
+  try auto with wf_db;
+  intros i j Hi Hj; simpl in *;
+  enumerate_matrix Hi Hj;
+  try lia;
+  try easy.
+
+  (* solve_matrix *)
+
+  
+
+Ltac bdestshoweq := (* goal of form b0 = b1, bools *)
+  match goal with 
+  | |- ?b0 = ?b1 =>
+    bdestruct b0; bdestruct b1; auto; try easy; lia
+  end.
+
+Ltac fail_if_iffy H :=
+  match H with
+  | context[if _ then _ else _] => fail 1
+  | _ => idtac
+  end.
+
+Ltac destruct_if :=
+  match goal with
+  | [ |- context[if ?b then _ else _]] 
+      => fail_if_iffy b; bdestruct b
+  end.
+
+Ltac destruct_if_solve :=
+  repeat (destruct_if; subst; tryeasylia);
+  tryeasylia.
+
+(* From: http://adam.chlipala.net/cpdt/html/Match.html *)
+
+Ltac notHyp P :=
+  match goal with
+    | [ _ : P |- _ ] => fail 1
+    | _ =>
+      match P with
+        | ?P1 /\ ?P2 => first [ notHyp P1 | notHyp P2 | fail 2 ]
+        | _ => idtac
+      end
+  end.
+
+(* Also from above source *)
+Ltac extend pf :=
+  let t := type of pf in
+    notHyp t; generalize pf; intro.
+
+Ltac add_mod_bound a n :=
+  let Han := fresh "Han" in assert(Han : a mod n < n)
+    by solve [apply Nat.mod_upper_bound; tryeasylia]; extend (Han).
+
+Ltac destruct_if_solve_mods :=
+  repeat (destruct_if; subst; tryeasylia);
+  repeat match goal with
+    | [ _ : context[?a mod ?n] |- _] => add_mod_bound a n
+    | [ |- context[?a mod ?n]] => add_mod_bound a n
+    end;
+  tryeasylia.
+
+
+
+Ltac apply_f H k :=
+  unfold compose in H;
+  apply (f_equal (fun x => x k)) in H.
+
+
+Lemma is_inv_iff_inv_is n f finv :
+  (forall k, k < n -> finv k < n /\ f k < n /\ f (finv k) = k /\ finv (f k) = k)%nat
+  <-> (forall k, k < n -> f k < n /\ finv k < n /\ finv (f k) = k /\ f (finv k) = k)%nat.
+Proof.
+  split; intros H k Hk; specialize (H k Hk); easy.
+Qed.
+
+
+#[export] Hint Rewrite is_inv_iff_inv_is : perm_inv_db.
+
+(* Tactic Notation "cleanup_perm_inv" := 
+  auto_cast_eqn (autorewrite with perm_inv_db).
+
+Tactic Notation "cleanup_perm" :=
+  auto_cast_eqn (autorewrite with perm_inv_db perm_cleanup_db).
+
+Tactic Notation "cleanup_perm_of_zx" :=
+  auto_cast_eqn (autorewrite with perm_of_zx_cleanup_db perm_inv_db perm_cleanup_db). *)
+
+
+Tactic Notation "cleanup_perm_inv" := 
+  autorewrite with perm_inv_db.
+
+Tactic Notation "cleanup_perm" :=
+  autorewrite with perm_inv_db perm_cleanup_db.
+
+Tactic Notation "cleanup_perm_of_zx" :=
+  autorewrite with perm_of_zx_cleanup_db perm_inv_db perm_cleanup_db.
+
+Lemma compose_id_of_compose_idn {f g : nat -> nat} 
+  (H : (f ∘ g)%prg = (fun n => n)) {k : nat} : f (g k) = k.
+Proof.
+  apply_f H k.
+  easy.
+Qed.
+
+Ltac perm_by_inverse finv :=
+  exists finv;
+  intros k Hk; repeat split;
+  only 3,4 : (try apply compose_id_of_compose_idn; cleanup_perm; tryeasylia) 
+            || cleanup_perm; tryeasylia;
+  only 1,2 : auto with perm_bdd_db; tryeasylia.
+
+
+
+
+Ltac solve_stack_perm n0 n1 :=
+  apply functional_extensionality; intros k;
+  unfold stack_perms;
+  bdestruct (k <? n0)%nat; [tryeasylia|];
+  try bdestruct (k <? n0 + n1)%nat; tryeasylia.
+  
+Ltac solve_stack_perm_strong n0 n1 :=
+  unfold stack_perms; 
+  apply functional_extensionality; intros k;
+  bdestruct (k <? n0)%nat; [tryeasylia | ]; try bdestruct (k <? n0 + n1);
+  destruct_if_solve.
+(* ^ REPLACED BY: solve_stack_perm; destruct_if_solve *)
+
+
+(* TODO: Figure out order of operations on where to put this vs its lemma *)
+(* Ltac by_inverse_injective f n :=
+  apply (WF_permutation_inverse_injective f n); [
+    tryeasylia; auto with perm_db |
+    tryeasylia; auto with perm_WF_db |
+    try solve [cleanup_perm; auto] |
+    try solve [cleanup_perm; auto]]; tryeasylia. *)
+
