src/Permutations/PermutationDefinitions.v
@@ -1,0 +1,45 @@
+Require Export QuantumLib.Permutations.
+Require Import CoreData.ZXCore.
+
+Notation idn := (fun (k : nat) => k).
+
+Fixpoint perm_inv n f : nat -> nat :=
+  fun k => match n with
+  | 0 => 0%nat
+  | S n' => if f n' =? k then n'%nat else perm_inv n' f k
+  end.
+
+Definition stack_perms (n0 n1 : nat) (f g : nat -> nat) : nat -> nat :=
+  fun n => 
+  if (n <? n0) then f n else 
+  if (n <? n0 + n1) then (g (n - n0) + n0)%nat else n.
+
+Definition swap_2_perm : nat -> nat :=
+  fun n => if 2 <=? n then n else match n with
+    | 0 => 1%nat
+    | 1 => 0%nat
+    | other => other
+  end.
+
+(* TODO: Combine the above and this? *)
+Definition swap_perm a b n := 
+  fun k => if n <=? k then k else 
+  if k =? a then b else
+  if k =? b then a else k.
+
+Definition rotr n m : nat -> nat :=
+	fun k => if n <=? k then k else (k + m) mod n.
+
+Definition rotl n m : nat -> nat :=
+	fun k => if n <=? k then k else (k + (n - (m mod n))) mod n.
+
+(* TODO: Refactor all with perm_WF *)
+Notation perm_WF n f := (forall k:nat, (n <= k)%nat -> f k = k).
+
+(* TODO: Implement things for this *)
+Fixpoint insertion_sort_list n f := 
+  match n with 
+  | 0 => []
+  | S n' => let k := (perm_inv (S n') f n') in
+      k :: insertion_sort_list n' (fswap f k n')
+  end.
