src/Permutations/PermutationInstances.v
@@ -1,0 +1,465 @@
+Require Export PermutationFacts.
+Require Import PermutationAutomation.
+Require Import ZXperm.
+
+
+Local Open Scope nat.
+Local Open Scope prg.
+
+
+
+Lemma idn_permutation : forall n, permutation n idn.
+Proof. exists idn. easy. Qed.
+
+Global Hint Resolve idn_permutation : perm_db.
+
+
+
+(* Section for swap_2_perm *)
+Lemma swap_2_perm_inv : 
+  swap_2_perm ∘ swap_2_perm = idn.
+Proof.
+  apply functional_extensionality; intros k.
+  repeat first [easy | destruct k].
+Qed.
+
+#[export] Hint Rewrite swap_2_perm_inv : perm_inv_db.
+
+Lemma swap_2_perm_bdd k :
+  k < 2 -> swap_2_perm k < 2.
+Proof.
+  intros Hk.
+  repeat first [easy | destruct k | cbn; lia].
+Qed.
+
+#[export] Hint Resolve swap_2_perm_bdd : perm_bdd_db.
+
+Lemma swap_2_perm_WF k : 1 < k -> swap_2_perm k = k.
+Proof.
+  intros. 
+  repeat first [easy | lia | destruct k].
+Qed.
+
+Global Hint Resolve swap_2_perm_WF : perm_WF_db.
+
+Lemma swap_2_perm_permutation : permutation 2 swap_2_perm.
+Proof. 
+  perm_by_inverse swap_2_perm.
+Qed.
+
+Global Hint Resolve swap_2_perm_permutation : perm_db.
+
+
+
+
+(* Section on swap_perm, swaps any two elements. TODO: Do we even want this?
+	 We have swap_2_perm and fswap... Also, should swap_perm be defined in 
+	 terms of fswap? *)
+Lemma swap_perm_same a n :
+  swap_perm a a n = idn.
+Proof.
+  unfold swap_perm.
+  apply functional_extensionality; intros k.
+  destruct_if_solve.
+Qed.
+
+#[export] Hint Rewrite swap_perm_same : perm_cleanup_db.
+
+Lemma swap_perm_comm a b n :
+  swap_perm a b n = swap_perm b a n.
+Proof.
+  apply functional_extensionality; intros k.
+  unfold swap_perm.
+  destruct_if_solve.
+Qed.
+
+Lemma swap_perm_WF a b n : forall k, n <= k -> swap_perm a b n k = k.
+Proof.
+  intros.
+  unfold swap_perm. 
+  destruct_if_solve.
+Qed.
+
+Global Hint Resolve swap_perm_WF : perm_WF_db.
+
+Lemma swap_perm_bdd a b n : a < n -> b < n ->
+  forall k, k < n -> swap_perm a b n k < n.
+Proof.
+  intros Ha Hb k Hk.
+  unfold swap_perm.
+  destruct_if_solve.
+Qed.
+
+Global Hint Resolve swap_perm_bdd : perm_bdd_db.
+
+Lemma swap_perm_inv a b n : a < n -> b < n -> 
+  (swap_perm a b n) ∘ (swap_perm a b n) = idn.
+Proof.
+  intros Ha Hb.
+  unfold compose.
+  apply functional_extensionality; intros k.
+  unfold swap_perm.
+  destruct_if_solve.
+Qed.
+
+#[export] Hint Rewrite swap_perm_inv : perm_inv_db.
+
+Lemma swap_perm_2_perm a b n : a < n -> b < n ->
+  permutation n (swap_perm a b n).
+Proof.
+  intros Ha Hb.
+  perm_by_inverse (swap_perm a b n).
+Qed.
+
+Global Hint Resolve swap_perm_2_perm : perm_db.
+
+Lemma swap_perm_S_permutation a n (Ha : S a < n) :
+  permutation n (swap_perm a (S a) n).
+Proof.
+  apply swap_perm_2_perm; lia.
+Qed.
+
+Global Hint Resolve swap_perm_S_permutation : perm_db.
+
+Lemma compose_swap_perm a b c n : a < n -> b < n -> c < n -> 
+  b <> c -> a <> c ->
+  (swap_perm a b n ∘ swap_perm b c n ∘ swap_perm a b n) = swap_perm a c n.
+Proof.
+  intros Ha Hb Hc Hbc Hac. 
+  apply functional_extensionality; intros k.
+  unfold compose, swap_perm.
+  destruct_if_solve.
+Qed.
+
+#[export] Hint Rewrite compose_swap_perm : perm_cleanup_db.
+
+
+
+
+
+(* Section for stack_perms *)
+Lemma stack_perms_WF_idn {n0 n1} {f} 
+	(H : forall k, n0 <= k -> f k = k): 
+	stack_perms n0 n1 f idn = f.
+Proof.
+	solve_stack_perm n0 n1;
+	rewrite H; lia.
+Qed.
+
+Lemma stack_perms_WF {n0 n1} {f g} k :
+  n0 + n1 <= k -> stack_perms n0 n1 f g k = k.
+Proof.
+  intros H.
+  unfold stack_perms.
+  destruct_if_solve.
+Qed.
+
+Global Hint Resolve stack_perms_WF : perm_WF_db.
+
+Lemma stack_perms_bdd {n0 n1} {f g}
+  (Hf : forall k, k < n0 -> f k < n0) (Hg : forall k, k < n1 -> g k < n1) :
+  forall k, k < n0 + n1 -> stack_perms n0 n1 f g k < n0 + n1.
+Proof.
+  intros k Hk.
+  unfold stack_perms.
+  bdestruct (k <? n0).
+  - specialize (Hf k H). lia.
+  - bdestruct (k <? n0 + n1); [|easy].
+    assert (Hkn0 : k - n0 < n1) by lia.
+    specialize (Hg _ Hkn0). lia.
+Qed. 
+
+Global Hint Resolve stack_perms_bdd : perm_bdd_db.
+
+Lemma stack_perms_rinv {n0 n1} {f g} {finv ginv}
+  (Hf: forall k, k < n0 -> (f k < n0 /\ finv k < n0 /\ finv (f k) = k /\ f (finv k) = k))
+  (Hg: forall k, k < n1 -> (g k < n1 /\ ginv k < n1 /\ ginv (g k) = k /\ g (ginv k) = k)) : 
+  stack_perms n0 n1 f g ∘ stack_perms n0 n1 finv ginv = idn.
+Proof.
+  unfold compose.
+  solve_stack_perm_strong n0 n1.
+  1-3: specialize (Hf _ H); lia.
+  - replace (ginv (k - n0) + n0 - n0) with (ginv (k - n0)) by lia.
+    assert (Hkn0: k - n0 < n1) by lia.
+    specialize (Hg _ Hkn0).
+    lia.
+  - assert (Hkn0: k - n0 < n1) by lia.
+    specialize (Hg _ Hkn0).
+    lia.
+Qed.
+
+Lemma stack_perms_linv {n0 n1} {f g} {finv ginv}
+  (Hf: forall k, k < n0 -> (f k < n0 /\ finv k < n0 /\ finv (f k) = k /\ f (finv k) = k))
+  (Hg: forall k, k < n1 -> (g k < n1 /\ ginv k < n1 /\ ginv (g k) = k /\ g (ginv k) = k)) : 
+  stack_perms n0 n1 finv ginv ∘ stack_perms n0 n1 f g = idn.
+Proof.
+  rewrite stack_perms_rinv.
+  2,3: rewrite is_inv_iff_inv_is.
+  all: easy.
+Qed.
+
+#[export] Hint Rewrite @stack_perms_rinv @stack_perms_linv : perm_inv_db.
+
+Lemma stack_perms_permutation {n0 n1 f g} (Hf : permutation n0 f) (Hg: permutation n1 g) :
+  permutation (n0 + n1) (stack_perms n0 n1 f g).
+Proof.
+  destruct Hf as [f' Hf'].
+  destruct Hg as [g' Hg'].
+  perm_by_inverse (stack_perms n0 n1 f' g').
+  1,2: apply stack_perms_bdd; try easy; intros k' Hk'; 
+       try specialize (Hf' _ Hk'); try specialize (Hg' _ Hk'); easy.
+  1,2: rewrite is_inv_iff_inv_is; easy.
+Qed.
+
+Global Hint Resolve stack_perms_permutation : perm_db.
+
+
+
+
+
+
+
+
+
+
+(* Section on rotr/rotl *)
+(* Lemma rotr_WF {n m} : 
+	forall k, n <= k -> (rotr n m) k = k.
+Proof. intros. unfold rotr. destruct_if; lia. Qed.
+
+Lemma rotl_WF {n m} : 
+	forall k, n <= k -> (rotl n m) k = k.
+Proof. intros. unfold rotl. destruct_if; lia. Qed.
+
+Global Hint Resolve rotr_WF rotl_WF : perm_WF_db.
+
+Lemma rotr_bdd {n m} : 
+	forall k, k < n -> (rotr n m) k < n.
+Proof.
+	intros. unfold rotr. destruct_if; [lia|].
+	apply Nat.mod_upper_bound; lia.
+Qed.
+
+Lemma rotl_bdd {n m} : 
+	forall k, k < n -> (rotl n m) k < n.
+Proof.
+	intros. unfold rotl. destruct_if; [lia|].
+	apply Nat.mod_upper_bound; lia.
+Qed.
+
+Global Hint Resolve rotr_bdd rotl_bdd : perm_bdd_db.
+
+Lemma rotr_rotl_inv n m :
+	((rotr n m) ∘ (rotl n m) = idn)%prg.
+Proof.
+	apply functional_extensionality; intros k.
+	unfold compose, rotl, rotr.
+	bdestruct (n <=? k); [destruct_if_solve|].
+	assert (Hn0 : n <> 0) by lia.
+	destruct_if.
+	- pose proof (Nat.mod_upper_bound (k + (n - m mod n)) n Hn0) as Hbad.
+	  lia. (* contradict Hbad *)
+	- rewrite Nat.add_mod_idemp_l; [|easy].
+	  rewrite <- Nat.add_assoc.
+	  replace (n - m mod n + m) with
+	    (n - m mod n + (n * (m / n) + m mod n)) by
+	    (rewrite <- (Nat.div_mod m n Hn0); easy).
+	  pose proof (Nat.mod_upper_bound m n Hn0).
+	  replace (n - m mod n + (n * (m / n) + m mod n)) with
+	    (n * (1 + m / n)) by lia.
+	  rewrite Nat.mul_comm, Nat.mod_add; [|easy].
+	  apply Nat.mod_small, H.
+Qed.
+
+Lemma rotl_rotr_inv n m : 
+	((rotl n m) ∘ (rotr n m) = idn)%prg.
+Proof.
+	apply functional_extensionality; intros k.
+	unfold compose, rotl, rotr.
+	bdestruct (n <=? k); [destruct_if_solve|].
+	assert (Hn0 : n <> 0) by lia.
+	destruct_if.
+	- pose proof (Nat.mod_upper_bound (k + m) n Hn0) as Hbad.
+	  lia. (* contradict Hbad *)
+	- rewrite Nat.add_mod_idemp_l; [|easy].
+	  rewrite <- Nat.add_assoc.
+	  replace (m + (n - m mod n)) with
+	    ((n * (m / n) + m mod n) + (n - m mod n)) by
+	    (rewrite <- (Nat.div_mod m n Hn0); easy).
+	  pose proof (Nat.mod_upper_bound m n Hn0).
+	  replace ((n * (m / n) + m mod n) + (n - m mod n)) with
+	    (n * (1 + m / n)) by lia.
+	  rewrite Nat.mul_comm, Nat.mod_add; [|easy].
+	  apply Nat.mod_small, H.
+Qed.
+
+#[export] Hint Rewrite rotr_rotl_inv rotl_rotr_inv : perm_inv_db.
+
+Lemma rotr_perm {n m} : permutation n (rotr n m).
+Proof. 
+	perm_by_inverse (rotl n m).
+Qed.
+
+Lemma rotl_perm {n m} : permutation n (rotl n m).
+Proof. 
+	perm_by_inverse (rotr n m).
+Qed.
+
+Global Hint Resolve rotr_perm rotl_perm : perm_db. *)
+
+
+
+
+
+
+
+
+
+
+
+
+
+
+
+
+
+(* Section on top_to_bottom and bottom_to_top *)
+Lemma bottom_to_top_perm_bdd {n} k : 
+	k < n -> bottom_to_top_perm n k < n.
+Proof.
+	intros Hk.
+	unfold bottom_to_top_perm.
+	bdest_lia_replace (n <=? k) false.
+	destruct k; lia.
+Qed.
+
+Lemma top_to_bottom_perm_bdd {n} k :
+	k < n -> top_to_bottom_perm n k < n.
+Proof.
+	intros Hk.
+	unfold top_to_bottom_perm.
+	bdest_lia_replace (n <=? k) false.
+	bdestruct (k =? n - 1); lia.
+Qed.
+
+Global Hint Resolve bottom_to_top_perm_bdd top_to_bottom_perm_bdd : perm_bdd_db.
+
+Lemma bottom_to_top_perm_WF {n} k : n <= k ->
+	bottom_to_top_perm n k = k.
+Proof.
+	intros Hk.
+	unfold bottom_to_top_perm.
+	bdest_lia_replace (n <=? k) true.
+	easy.
+Qed.
+
+Lemma top_to_bottom_perm_WF {n} k : n <= k ->
+	top_to_bottom_perm n k = k.
+Proof.
+	intros Hk.
+	unfold top_to_bottom_perm.
+	bdest_lia_replace (n <=? k) true.
+	easy.
+Qed.
+	
+Global Hint Resolve bottom_to_top_perm_WF top_to_bottom_perm_WF : perm_WF_db.
+
+Lemma bottom_to_top_to_bottom_inv n : 
+	bottom_to_top_perm n ∘ top_to_bottom_perm n = idn.
+Proof.
+	apply functional_extensionality; intros k.
+	unfold compose, bottom_to_top_perm, top_to_bottom_perm.
+	bdestruct (n <=? k).
+	1: bdest_lia_replace (n <=? k) true; easy.
+	bdestruct (k =? n - 1).
+	- destruct n.
+	  + easy.
+	  + bdest_lia_replace (S n <=? 0) false.
+	  	lia.
+	- bdest_lia_replace (n <=? k + 1) false.
+	  replace (k + 1) with (S k) by lia.
+	  easy.
+Qed.
+
+Lemma top_to_bottom_to_top_inv n :
+	top_to_bottom_perm n ∘ bottom_to_top_perm n = idn.
+Proof.
+	apply functional_extensionality; intros k.
+	unfold compose, bottom_to_top_perm, top_to_bottom_perm.
+	bdestruct (n <=? k).
+	1: bdest_lia_replace (n <=? k) true; easy.
+	destruct k.
+	- destruct n; [easy|].
+	  bdest_lia_replace (S n <=? S n - 1) false.
+	  rewrite Nat.eqb_refl.
+	  easy.
+	- bdest_lia_replace (n <=? k) false.
+	  bdest_lia_replace (k =? n - 1) false.
+	  lia.
+Qed.
+
+Lemma bottom_to_top_to_bottom_inv' {n k} :
+	bottom_to_top_perm n (top_to_bottom_perm n k) = k.
+Proof.
+	pose proof (bottom_to_top_to_bottom_inv n) as H.
+	apply (f_equal (fun g => g k)) in H.
+	unfold compose in H.
+	easy.
+Qed.
+
+Lemma top_to_bottom_to_top_inv' {n k} :
+	top_to_bottom_perm n (bottom_to_top_perm n k) = k.
+Proof.
+	pose proof (top_to_bottom_to_top_inv n) as H.
+	apply (f_equal (fun g => g k)) in H.
+	unfold compose in H.
+	easy.
+Qed.
+
+#[export] Hint Rewrite 
+  (fun n => @bottom_to_top_to_bottom_inv n)
+  (fun n => @bottom_to_top_to_bottom_inv' n)
+  (fun n => @top_to_bottom_to_top_inv n)
+  (fun n => @top_to_bottom_to_top_inv' n)
+  : perm_inv_db.
+
+
+Lemma top_to_bottom_permutation {n} :
+	permutation n (top_to_bottom_perm n).
+Proof.
+  perm_by_inverse (bottom_to_top_perm n).
+Qed.
+
+Lemma bottom_to_top_permutation {n} :
+	permutation n (bottom_to_top_perm n). 
+Proof.
+	perm_by_inverse (top_to_bottom_perm n).
+Qed.
+
+Global Hint Resolve top_to_bottom_permutation bottom_to_top_permutation : perm_db.
+
+
+Lemma top_to_bottom_perm_eq_rotr n :
+	top_to_bottom_perm n = rotr n 1.
+Proof.
+	apply functional_extensionality; intros k.
+	unfold top_to_bottom_perm, rotr.
+	destruct_if_solve.
+	- subst. 
+	  replace (n - 1 + 1) with n by lia.
+	  rewrite Nat.mod_same; lia.
+	- rewrite Nat.mod_small; lia.
+Qed.
+
+#[export] Hint Rewrite top_to_bottom_perm_eq_rotr : perm_cleanup_db.
+
+Lemma bottom_to_top_perm_eq_rotl n :
+	bottom_to_top_perm n = rotl n 1.
+Proof.
+  by_inverse_injective (top_to_bottom_perm n) n.
+Qed.
+
+#[export] Hint Rewrite bottom_to_top_perm_eq_rotl : perm_cleanup_db.
+
+Local Close Scope nat.
+Local Close Scope prg.
