src/Permutations/PermutationRules.v
@@ -1,0 +1,9 @@
+Require Export PermutationDefinitions.
+Require Export ZXperm.
+Require Export ZXpermSemantics.
+Require Export PermutationAutomation.
+Require Export ZXpermFacts.
+
+(* Horrible hack to fix scoping issues: *)
+Require Export StackComposeRules.
+
