src/Permutations/ZXpermFacts.v
@@ -1,0 +1,332 @@
+Require Import ZXCore.
+Require Import StackComposeRules.
+Require Import CastRules.
+Require Export ZXperm.
+Require Export ZXpermSemantics.
+Require Import PermutationAutomation.
+Require Export PermutationFacts.
+Require Export PermutationInstances. 
+
+(* In this file, we develop some tools for showing things are ZXperms and
+   prove some specific values of perm_of_zx *)
+
+
+
+(* Section on very general ZXperm facts *)
+
+Local Open Scope nat.
+
+Lemma zxperm_iff_cast {n0 n1 m0 m1} {zx} (Hn : n1 = n0) (Hm : m1 = m0) :
+	ZXperm n1 m1 (cast _ _ Hn Hm zx) <-> ZXperm n0 m0 zx.
+Proof.
+	split; intros; subst; easy.
+Qed.
+
+Global Hint Resolve <- zxperm_iff_cast : zxperm_db.
+
+Lemma cast_stack_zxperm {n0 n1 m0 m1 o p} {zx0} {zx1}
+	(H0 : ZXperm n0 m0 zx0) (H1 : ZXperm n1 m1 zx1) 
+	(Hn : o = n0 + n1) (Hm : p = m0 + m1) :
+	ZXperm o p (cast _ _ Hn Hm (zx0 ↕ zx1)).
+Proof.
+  auto with zxperm_db.
+Qed.
+
+Global Hint Resolve cast_stack_zxperm : zxperm_db.
+
+Lemma transpose_zxperm {n m} {zx} (H : ZXperm n m zx) :
+	ZXperm m n (zx ⊤).
+Proof.
+	induction H; simpl; constructor; try easy.
+Qed.
+
+Global Hint Resolve transpose_zxperm : zxperm_db.
+
+
+
+(* Section on core ZXperms *)
+Lemma n_wire_zxperm {n} : 
+	ZXperm n n (n_wire n).
+Proof.
+	induction n.
+	- constructor.
+	- simpl.
+    apply (PermStack PermWire IHn).
+Qed.
+
+Global Hint Resolve n_wire_zxperm : zxperm_db.
+
+Lemma n_compose_zxperm {n} {zx} (H : ZXperm n n zx) k :
+	ZXperm _ _ (n_compose k zx).
+Proof.
+	induction k; simpl; auto with zxperm_db.
+Qed.
+
+Global Hint Resolve n_compose_zxperm : zxperm_db.
+
+
+
+(* Section on specific ZXperms *)
+Lemma top_to_bottom_helper_zxperm n :
+	ZXperm (S n) (S n) (top_to_bottom_helper n).
+Proof.
+	induction n.
+	- constructor.
+	- simpl.
+	  constructor.
+	  + apply (PermStack PermSwap n_wire_zxperm).
+	  + apply (PermStack PermWire IHn).
+Qed.
+
+Global Hint Resolve top_to_bottom_helper_zxperm : zxperm_db.
+
+Lemma top_to_bottom_zxperm {n} :
+	ZXperm n n (top_to_bottom n).
+Proof.
+	destruct n; simpl; auto with zxperm_db.
+Qed.
+
+Lemma bottom_to_top_zxperm {n} :
+	ZXperm n n (bottom_to_top n).
+Proof.
+	apply transpose_zxperm.
+	apply top_to_bottom_zxperm.
+Qed.
+
+Global Hint Resolve top_to_bottom_zxperm bottom_to_top_zxperm : zxperm_db.
+
+
+
+
+
+
+
+
+
+
+
+
+
+
+
+
+
+
+(* Section on rules for perm_of_zx *)
+Lemma perm_of_zx_WF {n m} {zx} (H : ZXperm n m zx) : forall k, 
+	n <= k -> (perm_of_zx zx) k = k.
+Proof.
+	induction H; intros k Hk; try easy.
+	- simpl.
+	  destruct k; [|destruct k]; cbn; lia.
+	- simpl. 
+	  rewrite stack_perms_high; easy.
+	- simpl.
+	  unfold compose.
+	  pose proof (zxperm_square H).
+	  rewrite IHZXperm1; rewrite IHZXperm2; lia.
+	Qed.
+
+Global Hint Resolve perm_of_zx_WF : perm_WF_db.
+
+Lemma stack_perms_zx_idn {n0 m0 n1} {zx} (H : ZXperm n0 m0 zx) :
+	stack_perms n0 n1 (perm_of_zx zx) idn = 
+	perm_of_zx zx.
+Proof.
+	apply stack_perms_WF_idn.
+  auto with perm_WF_db.
+Qed.
+
+#[export] Hint Rewrite @stack_perms_zx_idn : perm_of_zx_cleanup_db.
+
+Lemma stack_perms_idn_zx {n0 n1 m1} {zx} (H : ZXperm n1 m1 zx) :
+	stack_perms n0 n1 idn (perm_of_zx zx) = 
+	fun k => if k <? n0 then k else (perm_of_zx zx (k - n0)) + n0.
+Proof.
+	solve_stack_perm n0 n1.
+	rewrite perm_of_zx_WF; [lia|easy|lia].
+Qed.
+
+Lemma perm_of_zx_compose_spec {n m o} {zx0 : ZX n m} {zx1 : ZX m o} :
+	perm_of_zx (zx0 ⟷ zx1) = 
+	(perm_of_zx zx0 ∘ perm_of_zx zx1)%prg.
+Proof. easy. Qed.
+
+Lemma perm_of_zx_stack_spec {n m o p} {zx0 : ZX n m} {zx1 : ZX o p} :
+	perm_of_zx (zx0 ↕ zx1) = 
+	stack_perms n o (perm_of_zx zx0) (perm_of_zx zx1).
+Proof. easy. Qed.
+
+Lemma perm_of_zx_cast {n m n' m'} {zx : ZX n' m'} 
+  (Hn : n = n') (Hm : m = m') :
+  perm_of_zx (cast _ _ Hn Hm zx) = perm_of_zx zx.
+Proof. subst. easy. Qed.
+
+#[export] Hint Rewrite 
+  @perm_of_zx_compose_spec
+  @perm_of_zx_stack_spec
+  @perm_of_zx_cast : perm_of_zx_cleanup_db.
+
+Lemma perm_of_transpose_is_rinv {n m} {zx} (H : ZXperm n m zx) :
+	(perm_of_zx zx ∘ perm_of_zx zx⊤)%prg = idn.
+Proof.
+	rewrite <- perm_of_zx_compose_spec.
+	induction H; apply functional_extensionality; intros k; try easy.
+	- cbn. 
+	  destruct k; [easy|destruct k; [easy|]].
+	  rewrite swap_2_perm_WF; rewrite swap_2_perm_WF; lia.
+	- simpl.
+    pose proof (zxperm_square H).
+    pose proof (zxperm_square H0).
+    subst.
+	  rewrite stack_perms_compose.
+	  2,3: auto with perm_db zxperm_db.
+	  rewrite <- 2!perm_of_zx_compose_spec.
+	  rewrite IHZXperm1, IHZXperm2; cleanup_perm.
+    easy.
+	- rewrite 2!perm_of_zx_compose_spec.
+	  simpl.
+	  rewrite <- Combinators.compose_assoc,
+	  	(Combinators.compose_assoc _ _ _ _ (perm_of_zx zx1 ⊤)).
+	  rewrite <- perm_of_zx_compose_spec, IHZXperm2, compose_idn_r.
+	  rewrite <- perm_of_zx_compose_spec, IHZXperm1.
+	  easy.
+Qed.
+
+Lemma perm_of_transpose_is_linv {n m} {zx} (H : ZXperm n m zx) :
+	(perm_of_zx zx⊤ ∘ perm_of_zx zx)%prg = idn.
+Proof.
+	pose proof (perm_of_transpose_is_rinv (transpose_zxperm H)) as Hinv.
+	rewrite <- transpose_involutive_eq in Hinv.
+	easy.
+Qed.
+
+#[export] Hint Rewrite 
+  @perm_of_transpose_is_rinv 
+  @perm_of_transpose_is_linv : perm_of_zx_cleanup_db.
+
+
+
+(* Section on specific values of perm_of_zx *)
+
+Lemma perm_of_n_wire n :
+	perm_of_zx (n_wire n) = idn.
+Proof.
+	induction n.
+	- easy.
+	- simpl.
+	  rewrite IHn.
+	  rewrite stack_perms_idn_idn.
+	  easy.
+Qed.
+
+#[export] Hint Rewrite perm_of_n_wire : perm_of_zx_cleanup_db.
+
+Lemma perm_of_zx_stack_n_wire {n0 m0} {zx} (H : ZXperm n0 m0 zx) {n1} :
+	perm_of_zx (zx ↕ (n_wire n1)) = perm_of_zx zx.
+Proof.
+	simpl.
+	rewrite perm_of_n_wire.
+	rewrite (stack_perms_zx_idn H).
+	easy. 
+Qed.
+
+#[export] Hint Rewrite @perm_of_zx_stack_n_wire : perm_of_zx_cleanup_db.
+
+Lemma perm_of_top_to_bottom_helper_eq {n} :
+	perm_of_zx (top_to_bottom_helper n) = top_to_bottom_perm (S n).
+Proof.
+	strong induction n; 
+	apply functional_extensionality; intros k.
+	destruct n; [destruct k; easy|].
+	simpl.
+	rewrite perm_of_n_wire.
+	rewrite stack_perms_WF_idn; [|apply swap_2_perm_WF].
+	rewrite stack_perms_idn_zx; [|apply top_to_bottom_helper_zxperm].
+	rewrite H; [|auto].
+	unfold compose.
+	bdestruct (k <? 1). 
+	- replace k with 0 by lia. easy.
+	- destruct n.
+	  1: destruct k; [easy|];
+	     destruct k; [easy|];
+		   cbn; destruct (k + 1) eqn:e; 
+       unfold swap_2_perm; destruct_if_solve.
+	  destruct k; [lia|].
+	  replace (S k - 1) with k by lia.
+	  unfold top_to_bottom_perm.
+	  replace (S (S (S n)) <=? S k) with (S (S n) <=? k) by bdestshoweq.
+	  replace (S k =? S (S (S n)) - 1) with (k =? S (S n) - 1) by bdestshoweq.
+	  bdestruct (S (S n) <=? k).
+	  + rewrite swap_2_perm_WF; lia.
+	  + bdestruct (k =? S (S n) - 1); [easy|].
+	    rewrite swap_2_perm_WF; lia.
+Qed.
+
+#[export] Hint Rewrite @perm_of_top_to_bottom_helper_eq : perm_of_zx_cleanup_db.
+
+Lemma perm_of_top_to_bottom_eq {n} :
+	perm_of_zx (top_to_bottom n) = top_to_bottom_perm n.
+Proof.
+	destruct n.
+	- apply functional_extensionality; intros k.
+	  easy.
+	- simpl.
+	  rewrite perm_of_top_to_bottom_helper_eq.
+	  easy.
+Qed.
+
+#[export] Hint Rewrite @perm_of_top_to_bottom_eq : perm_of_zx_cleanup_db.
+
+Lemma perm_of_bottom_to_top_eq n :
+	perm_of_zx (bottom_to_top n) = bottom_to_top_perm n.
+Proof.
+  by_inverse_injective (top_to_bottom_perm n) n.
+  rewrite <- perm_of_top_to_bottom_eq.
+	unfold bottom_to_top.
+  apply perm_of_transpose_is_linv; auto with zxperm_db.
+Qed.
+
+#[export] Hint Rewrite perm_of_bottom_to_top_eq : perm_of_zx_cleanup_db.
+
+Lemma perm_of_kcompose_top_to_bot_eq_rotr n k :
+	perm_of_zx (n_compose k (top_to_bottom n)) =
+	rotr n k.
+Proof.
+	induction k; simpl; try rewrite IHk; cleanup_perm_of_zx; easy.
+Qed.
+
+Lemma perm_of_kcompose_bot_to_top_eq_rotl n k :
+	perm_of_zx (n_compose k (bottom_to_top n)) =
+	rotl n k.
+Proof.
+	induction k; simpl; try rewrite IHk; cleanup_perm_of_zx; easy.
+Qed.
+
+#[export] Hint Rewrite 
+  perm_of_kcompose_top_to_bot_eq_rotr
+  perm_of_kcompose_bot_to_top_eq_rotl : perm_of_zx_cleanup_db.
+
+(* We can prove the rest (and really, whatever we want) easily. 
+   The main results are secitoned here so they don't overlap 
+   with the (same) proofs in SwapRules.v *)
+
+Lemma perm_of_top_to_bottom_1 n :
+	perm_of_zx (top_to_bottom (S n)) = perm_of_zx (n_compose n (bottom_to_top (S n))).
+Proof.
+  cleanup_perm_of_zx.
+	destruct n; [rewrite rotr_n, rotl_0_r; easy|].
+	rewrite rotr_eq_rotl_sub.
+	rewrite Nat.mod_small; [f_equal|]; lia.
+Qed.
+
+Lemma perm_of_n_compose_n_top_to_bottom n :
+	perm_of_zx (n_compose n (top_to_bottom n)) = perm_of_zx (n_wire n).
+Proof.
+	cleanup_perm_of_zx.
+	easy.
+Qed.
+
+#[export] Hint Rewrite perm_of_n_compose_n_top_to_bottom : perm_of_zx_cleanup_db.
+
+Local Close Scope nat.
