src/Permutations/ZXpermSemantics.v
@@ -1,0 +1,237 @@
+Require Import ZXCore.
+Require Import PermutationFacts.
+Require Import PermutationInstances.
+Require Import ZXperm.
+Require Import PermMatrix_temp. 
+Require Import PermutationAutomation.
+Require Import CoreData.Proportional.
+
+
+Local Open Scope nat. 
+
+(* First, we need this - which feels like it goes in ZXpermFacts, which
+   suggests the file structure is bad (probably because it is). *)
+Lemma zxperm_square {n m zx} : 
+  ZXperm n m zx -> n = m.
+Proof.
+  intros H.
+  induction H; subst; easy.
+Qed.
+
+Lemma zxperm_permutation n m zx : 
+  ZXperm n m zx -> permutation n (perm_of_zx zx).
+Proof. 
+  intros H.
+  induction H; show_permutation.
+- pose proof (zxperm_square H); pose proof (zxperm_square H0); subst.
+    simpl.
+    apply permutation_compose; easy.
+Qed.
+
+Global Hint Resolve zxperm_permutation : perm_db.
+
+Global Hint Resolve PermEmpty PermWire PermSwap PermStack PermComp : zxperm_db.
+
+(* TODO: Decide whether this goes here (it does) or somewhere else (it doesn't) *)
+Lemma stack_perms_matrix_helper {n0 n1 i j} {f g} (Hi : i < 2 ^ (n0 + n1)) (Hj: j < 2 ^ (n0 + n1)) :
+  permutation n0 f -> permutation n1 g ->
+  i =? qubit_perm_to_nat_perm (n0 + n1) (stack_perms n0 n1 f g) j = 
+  (i / 2 ^ n1 =? qubit_perm_to_nat_perm n0 f (j / 2 ^ n1)) &&
+  (i mod 2 ^ n1 =? qubit_perm_to_nat_perm n1 g (j mod 2 ^ n1)).
+Proof.
+  intros Hfperm Hgperm. 
+  pose proof Hfperm as [finv Hf].
+  pose proof Hgperm as [ginv Hg].
+  pose proof (stack_perms_permutation Hfperm Hgperm) as Hstackperm.
+  pose proof Hstackperm as [stackinv Hstack].
+  unfold qubit_perm_to_nat_perm.
+  rewrite eqb_iff, Bool.andb_true_iff, 3!Nat.eqb_eq.
+  split.
+  - intros Heq.
+    split.
+    + apply Nat.bits_inj.
+      intros k.
+      rewrite Heq, funbool_to_nat_div.
+      rewrite 2!nat_to_funbool_eq.
+      rewrite 2!testbit_funbool_to_nat.
+      bdestruct (k <? n0); [|easy].
+      unfold compose.
+      assert (Hlt:n0 - S k < n0) by lia.
+      replace (stack_perms n0 n1 f g (n0 - S k) <=? n0 + n1 - 1) with true by (
+        assert (Hlt2: n0 - S k < n0 + n1) by lia;
+        specialize (Hstack (n0 - S k) Hlt2);
+        bdestruct (stack_perms n0 n1 f g (n0 - S k) <=? n0 + n1 - 1); lia
+      ).
+      replace (f (n0 - S k) <=? n0 - 1) with true by (
+        specialize (Hf (n0 - S k) Hlt);
+        bdestruct (f (n0 - S k) <=? n0 - 1); lia
+      ).
+      unfold stack_perms.
+      replace (n0 - S k <? n0) with true by (bdestruct (n0 - S k <? n0); lia).
+      rewrite Nat.div_pow2_bits.
+      f_equal.
+      assert (S (f (n0 - S k)) <= n0). {
+        specialize (Hf (n0 - S k) Hlt).
+        lia. }
+      lia.
+    + apply Nat.bits_inj.
+      intros k.
+      rewrite Heq, funbool_to_nat_mod.
+      rewrite 2!nat_to_funbool_eq.
+      rewrite 2!testbit_funbool_to_nat.
+      bdestruct (k <? n1); [|easy].
+      unfold compose.
+      assert (Hlt:n1 - S k < n1) by lia.
+      rewrite Nat.mod_pow2_bits_low; [|lia].
+      unfold shift.
+      replace (stack_perms n0 n1 f g (n1 - S k + n0) <=? n0 + n1 - 1) with true by (
+        assert (Hlt2: n1 - S k + n0 < n0 + n1) by lia;
+        specialize (Hstack _ Hlt2);
+        bdestruct (stack_perms n0 n1 f g (n1 - S k + n0) <=? n0 + n1 - 1); lia
+      ).
+      replace (g (n1 - S k) <=? n1 - 1) with true by (
+        specialize (Hg (n1 - S k) Hlt);
+        bdestruct (g (n1 - S k) <=? n1 - 1); lia
+      ).
+      f_equal.
+      unfold stack_perms.
+      replace (n1 - S k + n0 <? n0) with false by (bdestruct (n1 - S k + n0 <? n0); lia).
+      replace (n1 - S k + n0 <? n0 + n1) with true by (bdestruct (n1 - S k + n0 <? n0 + n1); lia).
+      replace (n1 - S k + n0 - n0) with (n1 - S k) by lia.
+      lia.
+  - intros [Hdiv Hmod].
+    apply (div_mod_inj (2^n1)); [pose proof (Nat.pow_nonzero 2 n1); lia|].
+    split.
+    + rewrite Hmod.
+      rewrite funbool_to_nat_mod.
+      apply funbool_to_nat_eq.
+      intros k Hk.
+      rewrite shift_simplify.
+      unfold compose.
+      rewrite (stack_perms_right_add Hk).
+      
+      apply nat_to_funbool_mod.
+      specialize (Hg _ Hk); lia.
+    + rewrite Hdiv.
+      rewrite funbool_to_nat_div.
+      apply funbool_to_nat_eq.
+      intros k Hk.
+      unfold compose.
+      rewrite (stack_perms_left Hk).
+      apply nat_to_funbool_div.
+      specialize (Hf _ Hk); lia.
+Qed.
+
+
+
+Lemma empty_permutation_semantics : ⟦ Empty ⟧ = zxperm_to_matrix 0 Empty.
+Proof. check_finite_matrix. Qed.
+
+Lemma wire_permutation_semantics : ⟦ Wire ⟧ = zxperm_to_matrix 1 Wire.
+Proof. check_finite_matrix. Qed.
+
+Lemma swap_2_perm_semantics : ⟦ Swap ⟧ = zxperm_to_matrix 2 Swap.
+Proof. check_finite_matrix. Qed.
+
+Lemma apply_if2 {T1 T2 T3 : Type} {b1 b2 : bool} {x1 x2} {x3 x4} (f : T1 -> T2 -> T3) :
+  f (if b1 then x1 else x2) (if b2 then x3 else x4) = 
+  if b1 && b2 then f x1 x3 else (if b1 then f x1 x4 else (if b2 then f x2 x3 else f x2 x4)).
+Proof. destruct b1; destruct b2; easy. Qed.
+
+Lemma stack_perms_matrix {n0 n1 : nat} {f g : nat -> nat} :
+  permutation n0 f -> permutation n1 g ->
+  perm_to_matrix (n0 + n1) (stack_perms n0 n1 f g) =
+  (perm_to_matrix n0 f) ⊗ (perm_to_matrix n1 g).
+Proof.
+  intros Hf Hg.
+  apply mat_equiv_eq.
+  1,2:auto with wf_db.
+  intros i j Hi Hj.
+  
+  unfold kron, perm_to_matrix, perm_mat.
+  rewrite (proj2 (Nat.ltb_lt _ _) Hi), (proj2 (Nat.ltb_lt _ _) Hj).
+  replace (i / 2 ^ n1 <? 2 ^ n0) with true.
+  replace (j / 2 ^ n1 <? 2 ^ n0) with true.
+  replace (i mod 2 ^ n1 <? 2 ^ n1) with true.
+  replace (j mod 2 ^ n1 <? 2 ^ n1) with true.
+  repeat rewrite andb_true_r.
+  rewrite (apply_if2 Cmult), Cmult_0_l, Cmult_0_l, 
+  Cmult_1_l, Cmult_1_l, Tauto.if_same, Tauto.if_same.
+  rewrite (stack_perms_matrix_helper Hi Hj Hf Hg).
+  easy.
+  all: symmetry; rewrite Nat.ltb_lt.
+  1,2: apply Nat.mod_upper_bound; apply Nat.pow_nonzero; easy.
+  1,2: apply Nat.div_lt_upper_bound; try (apply Nat.pow_nonzero; easy).
+  1,2: rewrite Nat.pow_add_r, Nat.mul_comm in Hi, Hj; easy.
+Qed.
+
+Lemma stack_perms_semantics {n0 n1 m0 m1}
+  {zx0 : ZX n0 m0} {zx1 : ZX n1 m1} (H0 : n0 = m0) (H1 : n1 = m1) 
+  (Hzx0 : ⟦ zx0 ⟧ = zxperm_to_matrix n0 zx0) 
+  (Hzx1 : ⟦ zx1 ⟧ = zxperm_to_matrix n1 zx1) 
+  (Hzx0perm : permutation n0 (perm_of_zx zx0))
+  (Hzx1perm : permutation n1 (perm_of_zx zx1)) : 
+  ⟦ zx0 ↕ zx1 ⟧ = zxperm_to_matrix (n0 + n1) (zx0 ↕ zx1).
+Proof.
+  simpl.
+  rewrite stack_perms_matrix; [|easy|easy].
+  rewrite Hzx0, Hzx1.
+  subst.
+  easy.
+Qed.
+
+Lemma compose_permutation_semantics {n m o} {zx0 : ZX n m} {zx1 : ZX m o}
+  (H0 : n = m)
+  (Hzx0 : ⟦ zx0 ⟧ = zxperm_to_matrix n zx0)
+  (Hzx1 : ⟦ zx1 ⟧ = zxperm_to_matrix m zx1) 
+  (Hzx0perm : permutation n (perm_of_zx zx0))
+  (Hzx1perm : permutation m (perm_of_zx zx1)) :
+  ⟦ zx0 ⟷ zx1 ⟧ = zxperm_to_matrix n (zx0 ⟷ zx1).
+Proof.
+  cbn.
+  unfold perm_to_matrix.
+  rewrite <- qubit_perm_to_nat_perm_compose.
+  - rewrite <- perm_mat_Mmult.
+    + rewrite Hzx0, Hzx1.
+      subst; easy.
+    + apply qubit_perm_to_nat_perm_bij.
+      easy.
+  - subst; easy.
+Qed.
+
+Lemma cast_permutations_semantics {n0 m0 n1 m1} {zx : ZX n0 m0} 
+  (Hn : n1 = n0) (Hm : m1 = m0) 
+  (Hzx : ⟦ zx ⟧ = zxperm_to_matrix n1 zx) :
+  ⟦ cast _ _ Hn Hm zx ⟧ = zxperm_to_matrix n1 (cast _ _ Hn Hm zx).
+Proof. subst; easy. Qed.
+
+Lemma zxperm_permutation_semantics {n m zx} : 
+  ZXperm n m zx -> ⟦ zx ⟧ = zxperm_to_matrix n zx.
+Proof.
+  intros H.
+  induction H.
+  - apply empty_permutation_semantics.
+  - apply wire_permutation_semantics.
+  - apply swap_2_perm_semantics.
+  - eapply stack_perms_semantics; auto.
+    1,2: eapply zxperm_square; eassumption.
+    all: apply zxperm_permutation; easy.
+  - apply compose_permutation_semantics; auto.
+    1: eapply zxperm_square; eassumption.
+    all: apply zxperm_permutation; easy. 
+Qed.
+
+(* ... which enables the main result: *)
+
+Lemma prop_of_equal_perm {n m} {zx0 zx1 : ZX n m}
+	(Hzx0 : ZXperm n m zx0) (Hzx1 : ZXperm n m zx1)
+	(Hperm : perm_of_zx zx0 = perm_of_zx zx1) :
+	zx0 ∝ zx1.
+Proof.
+	prop_exists_nonzero (RtoC 1).
+	rewrite Mscale_1_l.
+	rewrite (zxperm_permutation_semantics Hzx0),
+		(zxperm_permutation_semantics Hzx1).
+	f_equal; easy.
+Qed.
+Local Close Scope nat. 
